Semantics

BasicConcrete.v
@@ -18,6 +18,7 @@ From Coq Require Import Init.Nat.
 From Coq Require Import Arith.Arith.
 From Coq Require Import Arith.EqNat. Import Nat.
 From Coq Require Import Init.Datatypes.
+From Coq Require Import Logic.FunctionalExtensionality. (* for equality of substitutions *)
 From SymEx Require Import BinaryRelation.
 
 Inductive Aexpr : Type :=
@@ -80,6 +81,12 @@ Fixpoint Bapply  (s:sub) (e:Bexpr) : Bexpr :=
 Definition update {E:Type} (s: string -> E) (x:string) (e:E) : string -> E :=
   fun y => if String.eqb x y then e else s x.
 
+Notation "x '!->' v ';' m" := (update m x v) (at level 100, v at next level, right associativity).
+Notation " x '!->' v " := (update id_sub x v) (at level 100, v at next level, right associativity).
+
+Definition empty_map {A:Type} (x:A) : string -> A := fun _ => x.
+Notation "'_' '!->' v" := (empty_map v) (at level 100, right associativity).
+
 Lemma Bapply_id : forall e,
     Bapply id_sub e = e.
 Proof.
@@ -127,14 +134,16 @@ Proof. intros. unfold Comp. unfold update. destruct (x =? y)%string;
          reflexivity.
 Qed.
 
+Lemma comp_id : forall V,
+    Comp V id_sub = V.
+Proof. intros. extensionality x. reflexivity. Qed.
+
 Inductive Stmt : Type :=
-| SSkip
 | SAsgn (x:string) (e:Aexpr)
 | SSeq (s1 s2:Stmt)
 | SIf (b:Bexpr) (s1 s2:Stmt)
 | SWhile (b:Bexpr) (s:Stmt).
 
-Notation "'skip'" := SSkip (in custom com at level 0) : com_scope.
 Notation "x := y"  :=
          (SAsgn x y)
             (in custom com at level 0, x constr at level 0,
@@ -146,14 +155,100 @@ Notation "'if' x '{' y '}' '{' z '}'" :=
          (SIf x y z)
            (in custom com at level 89, x at level 99,
             y at level 99, z at level 99) : com_scope.
+Notation "'while' x '{' y '}'" :=
+         (SWhile x y)
+           (in custom com at level 89, x at level 99,
+            y at level 99) : com_scope.
 
 (** Symbolic semantics *)
 
 Definition SConfig : Type := Stmt * sub * Bexpr.
 
-Reserved Notation " t '->s' t' " (at level 40).
+Reserved Notation " c '->s' c' " (at level 40).
 
 Inductive Sstep : Relation SConfig :=
 | SAsgn_step : forall s x e sig phi,
-    (<{ x := e ; s }>, sig , phi) ->s (s, (update sig x e), phi)
-  where " t '->s' t' " := (Sstep t t').
+    (<{ x := e ; s }>, sig , phi) ->s (s, (update sig x (Aapply sig e)), phi)
+| SIfTrue_step : forall b s1 s2 s sig phi,
+    (<{ if b {s1} {s2} ; s }>, sig, phi) ->s (<{ s1 ; s }>, sig, BAnd phi (Bapply sig b))
+| SIfFalse_step : forall b s1 s2 s sig phi,
+    (<{ if b {s1} {s2} ; s }>, sig, phi) ->s (<{ s1 ; s }>, sig, BAnd phi (BNot (Bapply sig b)))
+| SWhileTrue_step : forall b s s' sig phi,
+    (<{ while b {s} ; s' }>, sig, phi) ->s (<{ s ; while b {s} ; s' }>, sig, BAnd phi (Bapply sig b))
+| SWhileFalse_step : forall b s s' sig phi,
+    (<{ while b {s} ; s' }>, sig, phi) ->s (<{ s' }>, sig, BAnd phi (BNot (Bapply sig b)))
+  where " c '->s' c' " := (Sstep c c').
+
+Definition multi_Sstep := Trans_Ref_Closure Sstep.
+Notation " c '->*' c' " := (multi_Sstep c c') (at level 40).
+
+Example example_program : Stmt := <{ while (X <= 2) { X := X + 1 } ; Y := 1 }>.
+Example Sexample_run : (example_program, id_sub, BTrue)
+                        ->* (<{ Y := 1 }>, (X !-> <{X + 1 + 1}> ; X !-> <{X + 1}> ),
+                       <{ BTrue && X <= 2 && X + 1 <= 2 && ~ (X + 1 + 1 <= 2) }>).
+Proof. eapply Rstep. eapply Rstep. eapply Rstep. eapply Rstep. eapply Rstep. apply Rrefl.
+       apply SWhileTrue_step. apply SAsgn_step.
+       apply SWhileTrue_step. apply SAsgn_step.
+       apply SWhileFalse_step.
+Qed.
+
+Definition CConfig : Type := Stmt * Valuation.
+
+Reserved Notation " c '=>c' c'" (at level 40).
+
+Inductive Cstep : Relation CConfig :=
+| CAsgn_step : forall s x e V,
+    (<{ x := e ; s }>, V) =>c (s, update V x (Aeval V e))
+| CIfTrue_step : forall b s1 s2 s V,
+    Beval V b = true ->
+    (<{ if b {s1} {s2} ; s }>, V) =>c (<{ s1 ; s }>, V)
+| CIfFalse_step : forall b s1 s2 s V,
+    Beval V b = false ->
+    (<{ if b {s1} {s2} ; s }>, V) =>c (<{ s2 ; s }>, V)
+| CWhileTrue_step : forall b s s' V,
+    Beval V b = true ->
+    (<{ while b {s} ; s' }>, V) =>c (<{ s ; while b {s} ; s' }>, V)
+|CWhileFalse_step : forall b s s' V,
+    Beval V b = false ->
+    (<{ while b {s} ; s' }>, V) =>c (s' , V)
+where " c '=>c' c'" := (Cstep c c').
+
+Definition multi_Cstep := Trans_Ref_Closure Cstep.
+Notation " c '=>*' c' " := (multi_Cstep c c') (at level 40).
+
+Example example_V : Valuation := (_ !-> 1).
+Example Cexample_run : (example_program, example_V) =>* (<{ Y := 1 }>, (X !-> 3 ; X !-> 2 ; example_V)).
+Proof. eapply Rstep. eapply Rstep. eapply Rstep. eapply Rstep. eapply Rstep. apply Rrefl.
+       apply CWhileTrue_step. reflexivity.
+       apply CAsgn_step.
+       apply CWhileTrue_step. reflexivity.
+       apply CAsgn_step.
+       apply CWhileFalse_step. reflexivity.
+Qed.
+
+Lemma Sstep_end : forall c c',
+    c ->* c' ->
+    c = c' \/ exists c'', c ->* c'' /\ c'' ->s c'.
+Proof.
+  intros.
+  induction H.
+  - left. reflexivity.
+  - destruct IHTrans_Ref_Closure; right.
+    + exists y. rewrite H1. split.
+      * apply Rrefl.
+      * assumption.
+    + destruct H1 as [y' [Hcomp Hstep]].
+      exists y. split.
+      * apply Rstep with (y := y'); assumption.
+      * assumption.
+Qed.
+
+Lemma Cstep_combine : forall x y z,
+    x =>* y -> y =>c z -> x =>* z.
+Proof. intros. apply Rstep with (y := y); assumption. Qed.
+
+Theorem correctness : forall S S' sig phi V,
+    (S, id_sub, BTrue) ->* (S', sig, phi) ->
+    Beval V phi = true ->
+    (S, V) =>* (S', Comp V sig).
+Proof.
